adding prog

src/certigrad/aevb/graph.lean
@@ -9,43 +9,12 @@ import ..program ..prove_model_ok .util
 
 namespace certigrad
 namespace aevb
-/-
-section program
-open certigrad.program certigrad.program.statement certigrad.program.term certigrad.program.rterm list label
 
-@[cgsimp] def prog_naive : Π (a : arch) (x_data : T [a^.n_in, a^.n_x]), program | a x_data :=
-
-[
-input batch_start     [],
-param W_encode        [a^.ne, a^.n_in],
-param W_encode_μ      [a^.nz, a^.ne],
-param W_encode_logσ₂  [a^.nz, a^.ne],
-param W_decode        [a^.nd, a^.nz],
-param W_decode_p      [a^.n_in, a^.nd],
-
-assign x             $ get_col_range (const x_data) batch_start a^.bs,
-assign h_encode      $ softplus (gemm W_encode x),
-assign μ             $ gemm W_encode_μ h_encode,
-assign σ             $ sqrt (exp (gemm W_encode_logσ₂ h_encode)),
-sample z             $ mvn_iso μ σ,
-assign encoding_loss $ mvn_iso_empirical_kl μ σ z,
-assign p             $ sigmoid (gemm  W_decode_p (softplus (gemm W_decode z))),
-assign decoding_loss $ bernoulli_neglogpdf p x,
-
-cost encoding_loss,
-cost decoding_loss
-]
-
-end program
-
-@[cgsimp] def graph_naive : Π (a : arch) (x_data : T [a^.n_in, a^.n_x]), graph
-| a x_data := program_to_graph (prog_naive a x_data)
--/
 section nodes
 
-open det det.cwise1 det.cwise2 det.special rand.op label certigrad.tactic
+open det det.cwise1 det.cwise2 det.special rand.op label tactic certigrad.tactic
 
-@[cgsimp] def graph_naive : Π (a : arch) (x_data : T [a^.n_in, a^.n_x]), graph
+def graph_naive : Π (a : arch) (x_data : T [a^.n_in, a^.n_x]), graph
 | a x_data :=
 graph.mk [⟨(ID.nat 0, [a^.n_in, a^.n_x]), [], operator.det $ op.const x_data⟩,
           ⟨(ID.str x, [a^.n_in, a^.bs]), [(ID.nat 0, [a^.n_in, a^.n_x]), (ID.str batch_start, [])], operator.det $ op.special $ get_col_range _ _ _⟩,
@@ -67,9 +36,10 @@ graph.mk [⟨(ID.nat 0, [a^.n_in, a^.n_x]), [], operator.det $ op.const x_data�
           (ID.str W_decode, [a^.nd, a^.nz]), (ID.str W_decode_p, [a^.n_in, a^.nd])]
          [(ID.str batch_start, []), (ID.str W_encode, [a^.ne, a^.n_in]), (ID.str W_encode_μ, [a^.nz, a^.ne]),
           (ID.str W_encode_logσ₂, [a^.nz, a^.ne]), (ID.str W_decode, [a^.nd, a^.nz]), (ID.str W_decode_p, [a^.n_in, a^.nd])]
--- TODO(dhs): the following works (as of this writing) but is slow
--- by cgsimp
+
+attribute [cgsimp] graph_naive
 
 end nodes
+
 end aevb
 end certigrad
