src/certigrad/aevb/prog.lean
@@ -1,0 +1,45 @@
+/-
+Copyright (c) 2017 Daniel Selsam. All rights reserved.
+Released under Apache 2.0 license as described in the file LICENSE.
+Author: Daniel Selsam
+
+Certigrad code for a naive variational autoencoder.
+-/
+import ..program ..prove_model_ok .util .graph
+
+namespace certigrad
+namespace aevb
+
+section program
+open certigrad.program certigrad.program.statement certigrad.program.term certigrad.program.rterm list label
+
+def naive_aevb : Π (a : arch) (x_data : T [a^.n_in, a^.n_x]), graph | a x_data :=
+program_to_graph
+[
+input batch_start     [],
+param W_encode        [a^.ne, a^.n_in],
+param W_encode_μ      [a^.nz, a^.ne],
+param W_encode_logσ₂  [a^.nz, a^.ne],
+param W_decode        [a^.nd, a^.nz],
+param W_decode_p      [a^.n_in, a^.nd],
+
+assign x             $ get_col_range (const x_data) batch_start a^.bs,
+assign h_encode      $ softplus (gemm W_encode x),
+assign μ             $ gemm W_encode_μ h_encode,
+assign σ             $ sqrt (exp (gemm W_encode_logσ₂ h_encode)),
+sample z             $ mvn_iso μ σ,
+assign encoding_loss $ mvn_iso_empirical_kl μ σ z,
+assign p             $ sigmoid (gemm  W_decode_p (softplus (gemm W_decode z))),
+assign decoding_loss $ bernoulli_neglogpdf p x,
+
+cost encoding_loss,
+cost decoding_loss
+]
+
+end program
+
+@[cgsimp] lemma naive_aevb_as_graph (a : arch) (x_data : T [a^.n_in, a^.n_x]) : naive_aevb a x_data = graph_naive a x_data :=
+by { dunfold graph_naive naive_aevb, dcgsimp, cgsimp, reflexivity }
+
+end aevb
+end certigrad
